Integrate Wf and Interp proofs
Now the only admits remaining in Toplevel1 are glue ones about
freeze/to_bytes/from_bytes/fe_nonzero.  What remains (beyond those
admits, and the ones about word-by-word montgomery building blocks in
Arithmetic), are the proofs about abstract interpretation and the
rewriter.

After     | File Name                                                | Before    || Change    | % Change
--------------------------------------------------------------------------------------------------------
12m13.17s | Total                                                    | 11m45.42s || +0m27.75s | +3.93%
--------------------------------------------------------------------------------------------------------
3m47.20s  | Experiments/NewPipeline/Toplevel1                        | 3m27.51s  || +0m19.68s | +9.48%
0m17.98s  | Experiments/NewPipeline/UnderLetsProofs                  |    N/A    || +0m17.98s | ∞
   N/A    | Experiments/NewPipeline/UnderLetsWf                      | 0m17.94s  || -0m17.94s | -100.00%
4m49.57s  | Experiments/NewPipeline/SlowPrimeSynthesisExamples       | 4m45.22s  || +0m04.34s | +1.52%
1m16.28s  | Experiments/NewPipeline/Toplevel2                        | 1m13.33s  || +0m02.95s | +4.02%
0m02.96s  | Experiments/NewPipeline/MiscCompilerPassesProofs         |    N/A    || +0m02.96s | ∞
   N/A    | Experiments/NewPipeline/MiscCompilerPassesWf             | 0m02.91s  || -0m02.91s | -100.00%
0m58.32s  | Experiments/NewPipeline/Rewriter                         | 0m58.58s  || -0m00.25s | -0.44%
0m28.19s  | Experiments/NewPipeline/LanguageInversion                | 0m28.02s  || +0m00.17s | +0.60%
0m13.14s  | Experiments/NewPipeline/LanguageWf                       | 0m13.09s  || +0m00.05s | +0.38%
0m10.11s  | Experiments/NewPipeline/CStringification                 | 0m10.12s  || -0m00.00s | -0.09%
0m01.21s  | Experiments/NewPipeline/CLI                              | 0m01.19s  || +0m00.02s | +1.68%
0m01.11s  | Experiments/NewPipeline/StandaloneOCamlMain              | 0m01.13s  || -0m00.01s | -1.76%
0m01.09s  | Experiments/NewPipeline/GENERATEDIdentifiersWithoutTypes | 0m01.08s  || +0m00.01s | +0.92%
0m01.05s  | Experiments/NewPipeline/StandaloneHaskellMain            | 0m01.07s  || -0m00.02s | -1.86%
0m00.98s  | Experiments/NewPipeline/Language                         | 0m00.96s  || +0m00.02s | +2.08%
0m00.96s  | Experiments/NewPipeline/AbstractInterpretation           | 0m00.90s  || +0m00.05s | +6.66%
0m00.90s  | Experiments/NewPipeline/CompilersTestCases               | 0m00.92s  || -0m00.02s | -2.17%
0m00.66s  | Experiments/NewPipeline/RewriterProofs                   |    N/A    || +0m00.66s | ∞
0m00.64s  | Experiments/NewPipeline/MiscCompilerPasses               | 0m00.65s  || -0m00.01s | -1.53%
0m00.42s  | Experiments/NewPipeline/UnderLets                        | 0m00.38s  || +0m00.03s | +10.52%
0m00.40s  | Experiments/NewPipeline/AbstractInterpretationProofs     | 0m00.42s  || -0m00.01s | -4.76%

src/Experiments/NewPipeline/Language.v
@@ -143,6 +143,15 @@ Module Compilers.
          | arrow s d => fun x_xs y_ys => R s (fst x_xs) (fst y_ys) && @andb_bool_for_each_lhs_of_arrow _ f g R d (snd x_xs) (snd y_ys)
          end%bool.
 
+    Fixpoint and_for_each_lhs_of_arrow {base_type} {f g : type base_type -> Type}
+             (R : forall t, f t -> g t -> Prop)
+             {t}
+      : for_each_lhs_of_arrow f t -> for_each_lhs_of_arrow g t -> Prop
+      := match t with
+         | base t => fun _ _ => True
+         | arrow s d => fun x_xs y_ys => R s (fst x_xs) (fst y_ys) /\ @and_for_each_lhs_of_arrow _ f g R d (snd x_xs) (snd y_ys)
+         end.
+
     Section interpM.
       Context {base_type} (M : Type -> Type) (base_interp : base_type -> Type).
       (** half-monadic denotation function; denote [type]s into their
